Finish TreeSync.Level0 proofs

fstar/MLS.TreeSync.Level0.Proofs.fst
@@ -1,11 +1,14 @@
 module MLS.TreeSync.Level0.Proofs
 
 open Comparse
+open MLS.Crypto
+open MLS.NetworkTypes
 open MLS.Tree
 open MLS.TreeSync.NetworkTypes
 open MLS.TreeSync.Level0.Types
 open MLS.TreeSync.Level0
 open MLS.TreeSync.Level0.Invariants
+open MLS.TreeSync.ParentHash
 open MLS.TreeCommon
 
 #set-options "--fuel 1 --ifuel 1"
@@ -83,57 +86,72 @@ let rec unmerged_leaves_sorted_insert_sorted x l =
     else unmerged_leaves_sorted_insert_sorted x (z::t)
 #pop-options
 
-// TODO: unmerged_leaves_ok_add
+#push-options "--ifuel 2 --fuel 2"
+val mem_insert_sorted: x:nat_lbytes 4 -> l:list (nat_lbytes 4) -> elem:nat_lbytes 4 -> Lemma
+  (List.Tot.mem elem (insert_sorted x l) <==> elem == x \/ List.Tot.mem elem l)
+let rec mem_insert_sorted x l elem =
+  match l with
+  | [] -> ()
+  | [y] -> ()
+  | y::z::t ->
+    if x < y then ()
+    else if x = y then ()
+    else mem_insert_sorted x (z::t) elem
+#pop-options
 
-(*** External path ***)
-
-// TODO: unmerged_leaves_ok_apply_path
-
-  (*
-
-val leaf_at_add_: #l:nat -> #i:tree_index l -> t:treesync bytes tkt l i -> li:leaf_index l i{leaf_at t li == None} -> content:leaf_content -> li':leaf_index l i -> Lemma
-  (leaf_at (add_ t li content) li' = (if li = li' then Some content else leaf_at t li'))
-let rec leaf_at_add_ #l #i t li content li' =
+val leaf_at_tree_add: #bytes:Type0 -> {|bytes_like bytes|} -> #tkt:treekem_types bytes -> #l:nat -> #i:tree_index l -> t:treesync bytes tkt l i -> li:leaf_index l i{leaf_at t li == None} -> content:leaf_node_nt bytes tkt -> li':leaf_index l i -> Lemma
+  (requires tree_add_pre t li)
+  (ensures leaf_at (tree_add t li content) li' == (if li = li' then Some content else leaf_at t li'))
+let rec leaf_at_tree_add #bytes #bl #tkt #l #i t li content li' =
   match t with
   | TLeaf _ -> ()
   | TNode _ left right ->
     if is_left_leaf li && is_left_leaf li' then
-      leaf_at_add_ left li content li'
+      leaf_at_tree_add left li content li'
     else if not (is_left_leaf li) && not (is_left_leaf li') then
-      leaf_at_add_ right li content li'
+      leaf_at_tree_add right li content li'
     else ()
 
-val unmerged_leaves_ok_add_: #l:nat -> #i:tree_index l -> t:treesync bytes tkt l i -> li:leaf_index l i{leaf_at t li == None} -> content:leaf_content -> Lemma
-  (requires unmerged_leaves_ok t)
-  (ensures unmerged_leaves_ok (add_ t li content))
-let rec unmerged_leaves_ok_add_ #l #i t li content =
+val unmerged_leaves_ok_tree_add: #bytes:Type0 -> {|bytes_like bytes|} -> #tkt:treekem_types bytes -> #l:nat -> #i:tree_index l -> t:treesync bytes tkt l i -> li:leaf_index l i{leaf_at t li == None} -> content:leaf_node_nt bytes tkt -> Lemma
+  (requires tree_add_pre t li /\ unmerged_leaves_ok t)
+  (ensures unmerged_leaves_ok (tree_add t li content))
+let rec unmerged_leaves_ok_tree_add #bytes #bl #tkt #l #i t li content =
   match t with
   | TLeaf _ -> ()
   | TNode opt_content left right -> (
-    (if is_left_leaf li then unmerged_leaves_ok_add_ left li content else unmerged_leaves_ok_add_ right li content);
+    (if is_left_leaf li then unmerged_leaves_ok_tree_add left li content else unmerged_leaves_ok_tree_add right li content);
     match opt_content with
     | None -> ()
     | Some cont -> (
       list_for_all_eq (unmerged_leaf_exists t) cont.unmerged_leaves;
-      list_for_all_eq (unmerged_leaf_exists (add_ t li content)) (li::cont.unmerged_leaves);
-      introduce forall x. List.Tot.mem x (li::cont.unmerged_leaves) ==> Some? (leaf_at (add_ t li content) x)
+      list_for_all_eq (unmerged_leaf_exists (tree_add t li content)) (insert_sorted li cont.unmerged_leaves);
+      FStar.Classical.forall_intro (mem_insert_sorted li cont.unmerged_leaves);
+      unmerged_leaves_sorted_insert_sorted li cont.unmerged_leaves;
+      introduce forall x. List.Tot.mem x (insert_sorted li cont.unmerged_leaves) ==> Some? (leaf_at (tree_add t li content) x)
       with (
-        leaf_at_add_ t li content x
+        leaf_at_tree_add t li content x
       )
     )
   )
 
-val unmerged_leaves_ok_apply_valid_external_path_aux_: #l:nat -> #i:tree_index l -> t:treesync bytes tkt l i -> li:leaf_index l i -> p:valid_external_path t li -> parent_parent_hash:bytes -> Lemma
-  (requires unmerged_leaves_ok t)
-  (ensures unmerged_leaves_ok (apply_valid_external_path_aux_ t li p parent_parent_hash))
-let rec unmerged_leaves_ok_apply_valid_external_path_aux_ #l #i t li p parent_parent_hash =
+(*** External path ***)
+
+val unmerged_leaves_ok_apply_external_path_aux: #bytes:Type0 -> {|crypto_bytes bytes|} -> #tkt:treekem_types bytes -> #l:nat -> #i:tree_index l -> #li:leaf_index l i -> t:treesync bytes tkt l i -> p:external_pathsync bytes tkt l i li -> parent_parent_hash:mls_bytes bytes -> Lemma
+  (requires apply_external_path_aux_pre #bytes t p (length #bytes parent_parent_hash) /\ unmerged_leaves_ok t)
+  (ensures unmerged_leaves_ok (apply_external_path_aux t p parent_parent_hash))
+let rec unmerged_leaves_ok_apply_external_path_aux #bytes #cb #tkt #l #i #li t p parent_parent_hash =
   match t, p with
   | TLeaf _, PLeaf ext_content -> ()
   | TNode _ left right, PNode opt_ext_content p_next ->
     let (child, sibling) = get_child_sibling t li in
-    let (new_opt_content, new_parent_parent_hash) = apply_valid_external_path_aux_aux opt_ext_content sibling parent_parent_hash in
+    let (new_opt_content, new_parent_parent_hash) = compute_new_np_and_ph opt_ext_content sibling parent_parent_hash in
     if is_left_leaf li then
-      unmerged_leaves_ok_apply_valid_external_path_aux_ left li p_next new_parent_parent_hash
+      unmerged_leaves_ok_apply_external_path_aux left p_next new_parent_parent_hash
     else
-      unmerged_leaves_ok_apply_valid_external_path_aux_ right li p_next new_parent_parent_hash
-*)
+      unmerged_leaves_ok_apply_external_path_aux right p_next new_parent_parent_hash
+
+val unmerged_leaves_ok_apply_external_path: #bytes:Type0 -> {|crypto_bytes bytes|} -> #tkt:treekem_types bytes -> #l:nat -> #i:tree_index l -> #li:leaf_index l i -> t:treesync bytes tkt l i -> p:external_pathsync bytes tkt l i li -> Lemma
+  (requires apply_external_path_pre #bytes t p /\ unmerged_leaves_ok t)
+  (ensures unmerged_leaves_ok (apply_external_path t p))
+let unmerged_leaves_ok_apply_external_path #bytes #cb #tkt #l #i #li t p =
+  unmerged_leaves_ok_apply_external_path_aux t p (root_parent_hash #bytes)
